nsl/Security.ec
@@ -12,11 +12,14 @@ qed.
 (* ------------------------------------------------------------------------------------------ *)
 
 (* AEAD Reduction *)
-module (Red_AEAD (D : A_GWAKE) : A_GAEAD) (O : GAEAD_out) = {
+module (Red_AEAD_real (D : A_GWAKE) : A_GAEAD) (O : GAEAD_out) = {
   module WAKE_O : GWAKE_out = {
+    var b0 : bool
+
     var state_map: (id * int, role * instance_state) fmap
   
-    proc init_mem() : unit = {
+    proc init_mem(b: bool) : unit = {
+      b0 <- b;
       state_map <- empty;
     }
   
@@ -125,16 +128,202 @@ module (Red_AEAD (D : A_GWAKE) : A_GAEAD) (O : GAEAD_out) = {
       return ko;
     }
   
-    proc test = rev_skey
+    proc test(a, i) = {
+      var role, st, ps, k;
+      var ko <- None;
+ 
+      if ((a, i) \in state_map) {
+        (role, st) <- oget state_map.[(a, i)];
+        match st with
+        | Accepted trace k' => {
+          ps <- get_partners (a, i) (Some trace) role state_map;
+          if (card ps <= 1) {
+            ps <- get_observed_partners (a, i) state_map;
+            if (card ps = 0) {
+              if (b0 = false) {
+                k <- k';
+              } else {
+                k <$ dskey;
+              }
+              ko <- Some k;
+              state_map.[(a, i)] <- (role, Observed trace k);
+            }
+          }
+        }
+        | Observed _ _   => { }
+        | IPending _ _   => { }
+        | RPending _ _ _ => { }
+        | Aborted        => { }
+        end;
+      }
+      return ko;
+    }
   }
   
   proc run() = {
-    var b;
-    WAKE_O.init_mem();
-    b <@ D(WAKE_O).run();
-    return b;
+    var b';
+    WAKE_O.init_mem(false);
+    b' <@ D(WAKE_O).run();
+    return b';
   }
 }.
+
+module (Red_AEAD_ideal (D : A_GWAKE) : A_GAEAD) (O : GAEAD_out) = {
+  module WAKE_O : GWAKE_out = {
+    var b0 : bool
+
+    var state_map: (id * int, role * instance_state) fmap
+  
+    proc init_mem(b: bool) : unit = {
+      b0 <- b;
+      state_map <- empty;
+    }
+  
+    proc gen_pskey = O.gen
+  
+    proc send_msg1(a, i, b) = {
+      var ex, na;
+      var mo <- None;
+  
+      ex <@ O.ex((a, b));
+      if ((a, i) \notin state_map /\ ex) {
+        na <$ dnonce;
+        mo <@ O.enc((a, b), msg1_data a b, na);
+        state_map.[(a, i)] <- (Initiator, IPending (b, witness, na, oget mo) (a, oget mo));
+      }
+      return mo;
+    }
+
+    proc send_msg2(b, j, m1) = {
+      var a, ca, role, st, ex, n, nb;
+      var mo <- None;
+  
+      (a, ca) <- m1;
+      (role, st) <- oget state_map.[(b, j)];
+      ex <@ O.ex((a, b));
+      if ((b, j) \notin state_map /\ ex) {
+        n <@ O.dec((a, b), msg1_data a b, ca);
+        if (n is Some na) {
+          nb <$ dnonce;
+          mo <@ O.enc((a, b), msg2_data a b ca, nb);
+          state_map.[(b, j)] <- (Responder, RPending (a, witness, na, nb, ca, oget mo) m1 (oget mo));
+        } else {
+          state_map.[(b, j)] <- (Responder, Aborted);
+        }
+      }
+      return mo;
+    }
+
+    proc send_msg3(a, i, m2) = {
+      var role, st, b, psk, na, ca, n, skey, ok;
+      var mo <- None;
+  
+      if ((a, i) \in state_map) {
+        (role, st) <- oget state_map.[(a, i)];
+        if (st is IPending s m1) {
+          (b, psk, na, ca) <- s;
+          n <@ O.dec((a, b), msg2_data a b ca, m2);
+          if (n is Some nb) {
+            skey <- prf (na, nb) (a, b);
+            ok <$ dnonce;
+            mo <@ O.enc((a, b), msg3_data a b ca m2, ok);
+            state_map.[(a, i)] <- (Initiator, Accepted ((a, ca), m2, oget mo) skey);
+          } else {
+            state_map.[(a, i)] <- (Initiator, Aborted);
+          }
+        }
+      }
+      return mo;
+    }
+
+    proc send_fin(b, j, m3) = {
+      var role, st, a, psk, na, nb, ca, cb, ok, skey;
+      var mo <- None;
+
+      if ((b, j) \in state_map) {
+        (role, st) <- oget state_map.[(b, j)];
+        if (st is RPending s m1 m2) {
+          (a, psk, na, nb, ca, cb) <- s;
+          ok <@ O.dec((a, b), msg3_data a b ca cb, m3);
+          if (ok is Some nok) {
+            skey <- prf (na, nb) (a, b);
+            state_map.[(b, j)] <- (Responder, Accepted ((a, ca), cb, m3) skey);
+            mo <- Some ();
+          } else {
+            state_map.[(b, j)] <- (Responder, Aborted);
+          }
+        }
+      }
+      return mo;
+    }
+
+    proc rev_skey(a, i) = {
+      var role, st, ps, k;
+      var ko <- None;
+  
+      if ((a, i) \in state_map) {
+        (role, st) <- oget state_map.[(a, i)];
+        match st with
+        | Accepted trace k' => {
+          ps <- get_partners (a, i) (Some trace) role state_map;
+          if (card ps <= 1) {
+            ps <- get_observed_partners (a, i) state_map;
+            if (card ps = 0) {
+              k <- k';
+              ko <- Some k;
+              state_map.[(a, i)] <- (role, Observed trace k);
+            }
+          }
+        }
+        | Observed _ _   => { }
+        | IPending _ _   => { }
+        | RPending _ _ _ => { }
+        | Aborted        => { }
+        end;
+      }
+      return ko;
+    }
+  
+    proc test(a, i) = {
+      var role, st, ps, k;
+      var ko <- None;
+ 
+      if ((a, i) \in state_map) {
+        (role, st) <- oget state_map.[(a, i)];
+        match st with
+        | Accepted trace k' => {
+          ps <- get_partners (a, i) (Some trace) role state_map;
+          if (card ps <= 1) {
+            ps <- get_observed_partners (a, i) state_map;
+            if (card ps = 0) {
+              if (b0 = false) {
+                k <- k';
+              } else {
+                k <$ dskey;
+              }
+              ko <- Some k;
+              state_map.[(a, i)] <- (role, Observed trace k);
+            }
+          }
+        }
+        | Observed _ _   => { }
+        | IPending _ _   => { }
+        | RPending _ _ _ => { }
+        | Aborted        => { }
+        end;
+      }
+      return ko;
+    }
+  }
+  
+  proc run() = {
+    var b';
+    WAKE_O.init_mem(true);
+    b' <@ D(WAKE_O).run();
+    return b';
+  }
+}.
+
 
 (* ------------------------------------------------------------------------------------------ *)
 (* ROM Reduction *)
@@ -147,7 +336,7 @@ clone import PROM.FullRO as NROc with
   type d_out_t <= bool
 proof *.
 
-module (Red_ROM (D : A_GWAKE) : RO_Distinguisher) (O : RO) = {
+module (Red_ROM_real (D : A_GWAKE) : RO_Distinguisher) (O : RO) = {
   module WAKE_O : GWAKE_out = Game4 with {
     proc send_msg1 [
       ^if.^if.^na<$ ~ {na <- witness; O.sample((msg1_data a b, ca)); }
@@ -179,23 +368,65 @@ module (Red_ROM (D : A_GWAKE) : RO_Distinguisher) (O : RO) = {
   }
 
   proc distinguish() = {
-    var b;
-    WAKE_O.init_mem();
-    b <@ D(WAKE_O).run();
-    return b;
+    var b';
+    WAKE_O.init_mem(false);
+    b' <@ D(WAKE_O).run();
+    return b';
+  }
+}.
+
+module (Red_ROM_ideal (D : A_GWAKE) : RO_Distinguisher) (O : RO) = {
+  module WAKE_O : GWAKE_out = Game4 with {
+    proc send_msg1 [
+      ^if.^if.^na<$ ~ {na <- witness; O.sample((msg1_data a b, ca)); }
+    ]
+
+    proc send_msg2 [
+      ^if.^match#Some.^if.^nb<$ ~ {nb <- witness; O.sample((msg2_data a b ca, cb)); }
+    ]
+
+    proc send_msg3 [
+      ^if.^match#IPending.^match#Some.^if.^ok<$ ~ {
+        ok <- witness;
+        O.sample((msg3_data a b ca m2, caf));
+      }
+      ^if.^match#IPending.^match#Some.^if.^skey<- ~ {
+        na <@ O.get((msg1_data a b, ca));
+        ok <@ O.get((msg2_data a b ca, m2));
+        skey <- prf (na, ok) (a, b);
+      }
+    ]
+
+    proc send_fin [
+      ^if.^match#RPending.^match#Some.^skey<- ~ {
+        na <@ O.get((msg1_data a b, ca));
+        nb <@ O.get((msg2_data a b ca, cb));
+        skey <- prf (na, nb) (a, b);
+      }
+    ]
+  }
+
+  proc distinguish() = {
+    var b';
+    WAKE_O.init_mem(true);
+    b' <@ D(WAKE_O).run();
+    return b';
   }
 }.
 
 (* ------------------------------------------------------------------------------------------ *)
 (* PRF Reduction *)
-module (Red_PRF (D : A_GWAKE) : A_GPRF) (O : GPRF_out) = {
+module (Red_PRF_real (D : A_GWAKE) : A_GPRF) (O : GPRF_out) = {
   module WAKE_O : GWAKE_out = {
+    var b0 : bool
+
     var dec_map : ((id * id) * msg_data * ctxt, nonce) fmap
     var bad : bool
     var state_map : (id * int, role * instance_state) fmap
     var psk_map : (id * id, pskey) fmap
   
-    proc init_mem() = {
+    proc init_mem(b: bool) = {
+      b0 <- b;
       state_map <- empty;
       psk_map <- empty;
       bad <- false;
@@ -338,14 +569,236 @@ module (Red_PRF (D : A_GWAKE) : A_GPRF) (O : GPRF_out) = {
       return ko;
     }
   
-    proc test = rev_skey
+    proc test(a, i) = {
+      var role, st, ps, k;
+      var ko <- None;
+ 
+      if ((a, i) \in state_map) {
+        (role, st) <- oget state_map.[(a, i)];
+        match st with
+        | Accepted trace k' => {
+          ps <- get_partners (a, i) (Some trace) role state_map;
+          if (card ps <= 1) {
+            ps <- get_observed_partners (a, i) state_map;
+            if (card ps = 0) {
+              if (b0 = false) {
+                k <- k';
+              } else {
+                k <$ dskey;
+              }
+              ko <- Some k;
+              state_map.[(a, i)] <- (role, Observed trace k);
+            }
+          }
+        }
+        | Observed _ _   => { }
+        | IPending _ _   => { }
+        | RPending _ _ _ => { }
+        | Aborted        => { }
+        end;
+      }
+      return ko;
+    }
   }
   
   proc run() = {
-    var b;
-    WAKE_O.init_mem();
-    b <@ D(WAKE_O).run();
-    return b;
+    var b';
+    WAKE_O.init_mem(false);
+    b' <@ D(WAKE_O).run();
+    return b';
+  }
+}.
+
+module (Red_PRF_ideal (D : A_GWAKE) : A_GPRF) (O : GPRF_out) = {
+  module WAKE_O : GWAKE_out = {
+    var b0 : bool
+
+    var dec_map : ((id * id) * msg_data * ctxt, nonce) fmap
+    var bad : bool
+    var state_map : (id * int, role * instance_state) fmap
+    var psk_map : (id * id, pskey) fmap
+  
+    proc init_mem(b: bool) = {
+      b0 <- b;
+      state_map <- empty;
+      psk_map <- empty;
+      bad <- false;
+      dec_map <- empty;
+    }
+  
+    proc gen_pskey(a, b) = {
+      var k;
+  
+      if ((a, b) \notin psk_map) {
+        k <$ dpskey;
+        psk_map.[a, b] <- k;
+      }
+    }
+  
+    proc send_msg1(a, i, b) = {
+      var ca, mo;
+      
+      mo <- None;
+      if (((a, i) \notin state_map) /\ ((a, b) \in psk_map)) {
+        ca <$ dctxt;
+        bad <- bad \/ exists pk ad, (pk, ad, ca) \in dec_map;
+        if (!bad) {
+          dec_map.[(a, b), msg1_data a b, ca] <- witness;
+          mo <- Some ca;
+          state_map.[a, i] <- (Initiator, IPending (b, witness, witness, ca) (a, ca));
+        }
+      }
+      
+      return mo;
+    }
+
+    proc send_msg2(b : id, j : int, m1 : id * ctxt) : ctxt option = {
+      var a, ca, role, st, cb, mo;
+      
+      mo <- None;
+      (a, ca) <- m1;
+      (role, st) <- oget state_map.[b, j];
+      if (((b, j) \notin state_map) /\ ((a, b) \in psk_map)) {
+        if (dec_map.[(a, b), msg1_data a b, ca] is Some na) {
+          cb <$ dctxt;
+          bad <- bad \/ exists pk ad, (pk, ad, cb) \in dec_map;
+          if (!bad) {
+            dec_map.[(a, b), msg2_data a b ca, cb] <- witness;
+            mo <- Some cb;
+            state_map.[b, j] <- (Responder, RPending (a, witness, witness, witness, ca, cb) m1 cb);
+          }
+        } else {
+          state_map.[b, j] <- (Responder, Aborted);
+        }
+      }
+      
+      return mo;
+    }
+    
+    proc send_msg3(a : id, i : int, m2 : ctxt) : ctxt option = {
+      var role, st, b, psk, na, ca, skey, caf, mo; 
+      
+      mo <- None;
+      if ((a, i) \in state_map) {
+        (role, st) <- oget state_map.[a, i];
+        match (st) with
+        | IPending s m1 => {
+          (b, psk, na, ca) <- s;
+          if (dec_map.[(a, b), msg2_data a b ca, m2] is Some nb) {
+            caf <$ dctxt;
+            bad <- bad \/ exists pk ad, (pk, ad, caf) \in dec_map;
+            if (!bad) {
+              dec_map.[(a, b), msg3_data a b ca m2, caf] <- witness;
+              mo <- Some caf;
+              O.gen((msg3_data a b ca m2, caf));
+              skey <@ O.f((msg3_data a b ca m2, caf), (a, b));
+              state_map.[a, i] <- (Initiator, Accepted ((a, ca), m2, caf) (oget skey));
+            }
+          } else {
+            state_map.[a, i] <- (Initiator, Aborted);
+          }
+        }
+        | RPending _ _ _ => {}
+        | Accepted _ _ => {}
+        | Observed _ _ => {}
+        | Aborted => {}
+        end;
+      }
+      
+      return mo;
+    }
+
+    proc send_fin(b : id, j : int, m3 : ctxt) : unit option = {
+      var role, st, a, psk, na, nb, ca, cb, skey, mo;
+      
+      mo <- None;
+      if ((b, j) \in state_map) {
+        (role, st) <- oget state_map.[b, j];
+        match (st) with
+        | IPending _ _ => {}
+        | RPending s m1 m2 => {
+          (a, psk, na, nb, ca, cb) <- s;
+          if(dec_map.[(a, b), msg3_data a b ca cb, m3] is Some nok) {
+            skey <@ O.f((msg3_data a b ca cb, m3), (a, b));
+            state_map.[b, j] <- (Responder, Accepted ((a, ca), cb, m3) (oget skey));
+            mo <- Some tt;
+          } else {
+           state_map.[b, j] <- (Responder, Aborted);
+          }
+        }
+        | Accepted _ _ => {}
+        | Observed _ _ => {}
+        | Aborted => {}
+        end;
+      }
+      
+      return mo;
+    }
+
+    proc rev_skey(a, i) = {
+      var role, st, ps, k;
+      var ko <- None;
+  
+      if ((a, i) \in state_map) {
+        (role, st) <- oget state_map.[(a, i)];
+        match st with
+        | Accepted trace k' => {
+          ps <- get_partners (a, i) (Some trace) role state_map;
+          if (card ps <= 1) {
+            ps <- get_observed_partners (a, i) state_map;
+            if (card ps = 0) {
+              k <- k';
+              ko <- Some k;
+              state_map.[(a, i)] <- (role, Observed trace k);
+            }
+          }
+        }
+        | Observed _ _   => { }
+        | IPending _ _   => { }
+        | RPending _ _ _ => { }
+        | Aborted        => { }
+        end;
+      }
+      return ko;
+    }
+  
+    proc test(a, i) = {
+      var role, st, ps, k;
+      var ko <- None;
+ 
+      if ((a, i) \in state_map) {
+        (role, st) <- oget state_map.[(a, i)];
+        match st with
+        | Accepted trace k' => {
+          ps <- get_partners (a, i) (Some trace) role state_map;
+          if (card ps <= 1) {
+            ps <- get_observed_partners (a, i) state_map;
+            if (card ps = 0) {
+              if (b0 = false) {
+                k <- k';
+              } else {
+                k <$ dskey;
+              }
+              ko <- Some k;
+              state_map.[(a, i)] <- (role, Observed trace k);
+            }
+          }
+        }
+        | Observed _ _   => { }
+        | IPending _ _   => { }
+        | RPending _ _ _ => { }
+        | Aborted        => { }
+        end;
+      }
+      return ko;
+    }
+  }
+  
+  proc run() = {
+    var b';
+    WAKE_O.init_mem(true);
+    b' <@ D(WAKE_O).run();
+    return b';
   }
 }.
 
@@ -367,7 +820,7 @@ module Counter (W : GWAKE_out) : GWAKE_out_i = {
 
   include W[send_fin, gen_pskey, test, rev_skey]
 
-  proc init_mem() = {
+  proc init_mem(b: bool) = {
     (cm1, cm2, cm3) <- (0, 0, 0);
   }
   
@@ -405,11 +858,20 @@ module Red_Coll_O_WAKE (S : BD.ASampler) = Game2 with {
   ]
 }.
 
-module (Red_Coll (A : A_GWAKE) : BD.Adv) (S : BD.ASampler) = {
+module (Red_Coll_real (A : A_GWAKE) : BD.Adv) (S : BD.ASampler) = {
   proc a() = {
     var b;
-    Red_Coll_O_WAKE(S).init_mem();
-    Counter(Red_Coll_O_WAKE(S)).init_mem();
+    Red_Coll_O_WAKE(S).init_mem(false);
+    Counter(Red_Coll_O_WAKE(S)).init_mem(false);
+    b <@ A(Counter(Red_Coll_O_WAKE(S))).run();
+  }
+}.
+
+module (Red_Coll_ideal (A : A_GWAKE) : BD.Adv) (S : BD.ASampler) = {
+  proc a() = {
+    var b;
+    Red_Coll_O_WAKE(S).init_mem(true);
+    Counter(Red_Coll_O_WAKE(S)).init_mem(true);
     b <@ A(Counter(Red_Coll_O_WAKE(S))).run();
   }
 }.
@@ -417,6 +879,7 @@ module (Red_Coll (A : A_GWAKE) : BD.Adv) (S : BD.ASampler) = {
 (* ------------------------------------------------------------------------------------------ *)
 (* ROM Reduction skeys *)
 
+(*
 clone PROM.FullRO as KROc with
   type in_t    <= trace,
   type out_t   <= skey,
@@ -439,7 +902,7 @@ module (Red_ROM_sk_1 (D : A_GWAKE) : KROc.RO_Distinguisher) (O : KROc.RO) = {
     ]
 
     proc test [
-      ^if.^match#Accepted.^if.^if.^k<- ~ { k <@ O.get(trace); }
+      ^if.^match#Accepted.^if.^if.^if.^k<- ~ { k <@ O.get(trace); }
     ]
   }
 
@@ -479,13 +942,13 @@ module (Red_ROM_sk_2 (D : A_GWAKE) : KROc.RO_Distinguisher) (O : KROc.RO) = {
     b <@ D(WAKE_O).run();
     return b;
   }
-}.
+}.*)
 (* ------------------------------------------------------------------------------------------ *)
 (* Security Proof *)
 (* ------------------------------------------------------------------------------------------ *)
 section.
 
-declare module A <: A_GWAKE {-GWAKE0, -Game1, -Game2, -Game3, -Game4, -Game5, -Game6, -Game7, -Game8, -GAEAD0, -GAEAD1, -PRF0, -PRF1, -Red_AEAD, -Red_Coll, -Red_ROM, -Red_PRF, -Red_ROM_sk_1, -Red_ROM_sk_2, -RO, -FRO, -KROc.RO, -KROc.FRO, -BD.Sample}.
+declare module A <: A_GWAKE {-GWAKEb, -Game1, -Game2, -Game3, -Game4, -Game5, -Game6, -Game7, -Game8, -GAEAD0, -GAEAD1, -PRF0, -PRF1, -Red_AEAD_real, -Red_AEAD_ideal, -Red_Coll_real, -Red_Coll_ideal, -Red_ROM_real, -Red_ROM_ideal, -Red_PRF_real, -Red_PRF_ideal, -RO, -FRO, -BD.Sample}.
 
 declare axiom A_ll:
 forall (GW <: GWAKE_out{-A}),
@@ -504,10 +967,10 @@ lemma obs_ps sm h h' s:
 proof.
 admitted.
 
+
+(*
 (* ------------------------------------------------------------------------------------------ *)
 (* Step 7 aux: Show the two reductions on sk are equivalent *)
-print KROc.RO.
-
 
 inductive Game7_inv 
   (sm: (id * int, role * instance_state) fmap)
@@ -882,7 +1345,7 @@ call(: ={state_map, psk_map, dec_map, bad, prfkey_map}(Red_ROM_sk_2.WAKE_O, Game
 
 auto=> />.
 smt(emptyE).
-qed.
+qed.*)
 
 (* ------------------------------------------------------------------------------------------ *)
 (* Step 0: Inline procedure calls, and remove pskeys from the state using psk_map to retrieve. *)
@@ -928,27 +1391,27 @@ case: (sml.[h])=> //.
 by move=> [r' []] // [].
 qed.
 
-lemma Step0 &m:
-    Pr[E_GWAKE(GWAKE0(NSL), A).run() @ &m : res] = Pr[E_GWAKE(Game1, A).run() @ &m : res].
+lemma Step0 bit &m:
+    Pr[E_GWAKE(GWAKEb(NSL), A).run(bit) @ &m : res] = Pr[E_GWAKE(Game1, A).run(bit) @ &m : res].
 proof.
 byequiv => //.
 proc; inline*.
 call (:
-    ={psk_map}(GWAKEb, Game1)
+    ={b0, psk_map}(GWAKEb, Game1)
 /\ (forall h, omap (fun v => let (r, s) = v in (r, clear_psk s)) GWAKEb.state_map.[h]{1} = Game1.state_map.[h]{2})
-/\ (forall a i, GWAKE0_inv GWAKEb.state_map GWAKEb.psk_map a i){1}
+/\ (forall a i, GWAKEb_inv GWAKEb.state_map GWAKEb.psk_map a i){1}
 ).
 - conseq (: ={res}
-          /\ ={psk_map}(GWAKEb, Game1)
+          /\ ={b0, psk_map}(GWAKEb, Game1)
           /\ (forall h, omap (fun v => let (r, s) = v in (r, clear_psk s)) GWAKEb.state_map.[h]{1} = Game1.state_map.[h]{2})
-  ) GWAKE0_inv_gen_pskey _ => //.
+  ) GWAKEb_inv_gen_pskey _ => //.
   proc.
   by if; auto.
 
 - conseq (: ={res}
-          /\ ={psk_map}(GWAKEb, Game1)
+          /\ ={b0, psk_map}(GWAKEb, Game1)
           /\ (forall h, omap (fun v => let (r, s) = v in (r, clear_psk s)) GWAKEb.state_map.[h]{1} = Game1.state_map.[h]{2})
-  ) GWAKE0_inv_send_msg1 _ => //.
+  ) GWAKEb_inv_send_msg1 _ => //.
   proc; inline.
   sp; wp; if=> //.
   + smt().
@@ -956,9 +1419,9 @@ call (:
   smt(get_setE).
 
 - conseq (: ={res}
-          /\ ={psk_map}(GWAKEb, Game1)
+          /\ ={b0, psk_map}(GWAKEb, Game1)
           /\ (forall h, omap (fun v => let (r, s) = v in (r, clear_psk s)) GWAKEb.state_map.[h]{1} = Game1.state_map.[h]{2})
-  ) GWAKE0_inv_send_msg2 _ => //.
+  ) GWAKEb_inv_send_msg2 _ => //.
   proc; inline.
   sp; wp; if=> //.
   + smt().
@@ -970,9 +1433,9 @@ call (:
   by match Some {1} ^match; auto; smt(get_setE).
 
 - conseq (: ={res}
-          /\ ={psk_map}(GWAKEb, Game1)
+          /\ ={b0, psk_map}(GWAKEb, Game1)
           /\ (forall h, omap (fun v => let (r, s) = v in (r, clear_psk s)) GWAKEb.state_map.[h]{1} = Game1.state_map.[h]{2})
-  ) GWAKE0_inv_send_msg3 _ => //.
+  ) GWAKEb_inv_send_msg3 _ => //.
   proc; inline.
   sp; wp; if=> //.
   + smt().
@@ -998,9 +1461,9 @@ call (:
   smt(get_setE).
 
 - conseq (: ={res}
-          /\ ={psk_map}(GWAKEb, Game1)
+          /\ ={b0, psk_map}(GWAKEb, Game1)
           /\ (forall h, omap (fun v => let (r, s) = v in (r, clear_psk s)) GWAKEb.state_map.[h]{1} = Game1.state_map.[h]{2})
-  ) GWAKE0_inv_send_fin _ => //.
+  ) GWAKEb_inv_send_fin _ => //.
   proc; inline.
   sp; wp ^if ^if; if=> //.
   + smt().
@@ -1026,9 +1489,9 @@ call (:
   smt(get_setE).
 
 - conseq (: ={res}
-          /\ ={psk_map}(GWAKEb, Game1)
+          /\ ={b0, psk_map}(GWAKEb, Game1)
           /\ (forall h, omap (fun v => let (r, s) = v in (r, clear_psk s)) GWAKEb.state_map.[h]{1} = Game1.state_map.[h]{2})
-  ) GWAKE0_inv_rev_skey _ => //.
+  ) GWAKEb_inv_rev_skey _ => //.
   proc; inline. 
   sp; wp ^if ^if; if=> //.
   + smt().
@@ -1054,11 +1517,10 @@ call (:
   smt(get_set_sameE). 
   do rewrite get_set_neqE => //. rewrite eqsm => //.
 
-
 - conseq (: ={res}
-          /\ ={psk_map}(GWAKEb, Game1)
+          /\ ={b0, psk_map}(GWAKEb, Game1)
           /\ (forall h, omap (fun v => let (r, s) = v in (r, clear_psk s)) GWAKEb.state_map.[h]{1} = Game1.state_map.[h]{2})
-     ) GWAKE0_inv_test _ => //.
+     ) GWAKEb_inv_test _ => //.
   proc; inline. 
   sp; wp ^if ^if; if=> //.
   + smt().
@@ -1075,29 +1537,36 @@ call (:
   sp ^if & -1 ^if & -1; if=> //.
   + move => &1 &2 [] /> *.
     by rewrite (eq_obs_partners (a, i){2} GWAKEb.state_map{1} Game1.state_map{2}) => //.
-  auto=> /> &1 &2 + + eqsm invl a_in _.
+  if => //.  
+  + auto=> /> &1 &2 + + eqsm invl a_in _.
+    rewrite -(eqsm (a, i){2}).
+    move => *.
+    split. smt().
+    move => h.
+    case (h = (a, i){2}) => [|hneq].
+    + smt(get_set_sameE). 
+    do rewrite get_set_neqE => //. rewrite eqsm => //.
+  auto=> /> &1 &2 + + eqsm invl a_in _ _ ideal sk _.
   rewrite -(eqsm (a, i){2}).
-  move => *.
-  split. smt().
-  move => h.
+  move => stm1 stm2 h.
   case (h = (a, i){2}) => [|hneq].
-  smt(get_set_sameE). 
+  + smt(get_set_sameE). 
   do rewrite get_set_neqE => //. rewrite eqsm => //.
 
 auto=> />.
 split; 1: smt(emptyE).
 move=> a i. 
-apply GWAKE0_undef.
+apply GWAKEb_undef.
 smt(emptyE).
 qed.
 
 (* ------------------------------------------------------------------------------------------ *)
 (* Step 1: Apply the AEAD assumption. *)
 
-lemma Step1 &m:
-    `|Pr[E_GWAKE(Game1, A).run() @ &m : res] - Pr[E_GWAKE(Game2, A).run() @ &m : res]|
+lemma Step1_real &m:
+    `|Pr[E_GWAKE(Game1, A).run(false) @ &m : res] - Pr[E_GWAKE(Game2, A).run(false) @ &m : res]|
   = 
-    `|Pr[E_GAEAD(GAEAD0, Red_AEAD(A)).run() @ &m : res] - Pr[E_GAEAD(GAEAD1, Red_AEAD(A)).run() @ &m : res]|.
+    `|Pr[E_GAEAD(GAEAD0, Red_AEAD_real(A)).run() @ &m : res] - Pr[E_GAEAD(GAEAD1, Red_AEAD_real(A)).run() @ &m : res]|.
 proof.
 do! congr.
 + byequiv => //.
@@ -1105,19 +1574,19 @@ do! congr.
   wp.
   call (:
         ={psk_map}(Game1, GAEADb)
-     /\ ={state_map}(Game1, Red_AEAD.WAKE_O)
+     /\ ={b0, state_map}(Game1, Red_AEAD_real.WAKE_O)
      /\ (forall a i, Game1_inv Game1.state_map Game1.psk_map a i){1}
   )=> //.
 
   - conseq (: ={res}
          /\ ={psk_map}(Game1, GAEADb)
-         /\ ={state_map}(Game1, Red_AEAD.WAKE_O)
+         /\ ={b0, state_map}(Game1, Red_AEAD_real.WAKE_O)
     ) Game1_inv_gen_pskey _ => //.
     by proc; if; auto.
 
   - conseq (: ={res}
          /\ ={psk_map}(Game1, GAEADb)
-         /\ ={state_map}(Game1, Red_AEAD.WAKE_O)
+         /\ ={b0, state_map}(Game1, Red_AEAD_real.WAKE_O)
     ) Game1_inv_send_msg1 _ => //.
     proc; inline.
     sp; wp; if=> //.
@@ -1125,7 +1594,7 @@ do! congr.
 
   - conseq (: ={res}
          /\ ={psk_map}(Game1, GAEADb)
-         /\ ={state_map}(Game1, Red_AEAD.WAKE_O)
+         /\ ={b0, state_map}(Game1, Red_AEAD_real.WAKE_O)
     ) Game1_inv_send_msg2 _ => //.
     proc; inline.
     sp; wp; if=> //.
@@ -1139,7 +1608,7 @@ do! congr.
 
   - conseq (: ={res}
          /\ ={psk_map}(Game1, GAEADb)
-         /\ ={state_map}(Game1, Red_AEAD.WAKE_O)
+         /\ ={b0, state_map}(Game1, Red_AEAD_real.WAKE_O)
     ) Game1_inv_send_msg3 _ => //.
     proc; inline.
     sp; wp; if=> //.
@@ -1160,7 +1629,7 @@ do! congr.
 
   - conseq (: ={res}
          /\ ={psk_map}(Game1, GAEADb)
-         /\ ={state_map}(Game1, Red_AEAD.WAKE_O)
+         /\ ={b0, state_map}(Game1, Red_AEAD_real.WAKE_O)
     ) Game1_inv_send_fin _ => //.
     proc; inline.
     sp; wp ^if ^if; if=> //.
@@ -1175,13 +1644,13 @@ do! congr.
 
   - conseq (: ={res}
          /\ ={psk_map}(Game1, GAEADb)
-         /\ ={state_map}(Game1, Red_AEAD.WAKE_O)
+         /\ ={b0, state_map}(Game1, Red_AEAD_real.WAKE_O)
     ) Game1_inv_rev_skey _ => //.
     by sim.
 
   - conseq (: ={res}
          /\ ={psk_map}(Game1, GAEADb)
-         /\ ={state_map}(Game1, Red_AEAD.WAKE_O)
+         /\ ={b0, state_map}(Game1, Red_AEAD_real.WAKE_O)
     ) Game1_inv_test _ => //.
     by sim. 
   
@@ -1194,13 +1663,13 @@ proc; inline*.
 wp.
 call (:
       ={psk_map}(Game2, GAEADb)
-      /\ ={state_map}(Game2, Red_AEAD.WAKE_O)
+      /\ ={b0, state_map}(Game2, Red_AEAD_real.WAKE_O)
       /\ Game2.dec_map{1} = GAEAD1.ctxts{2}
       /\ (forall a i, Game1_inv Game2.state_map Game2.psk_map a i){1}
 ).
 - conseq (: ={res}
        /\ ={psk_map}(Game2, GAEADb)
-       /\ ={state_map}(Game2, Red_AEAD.WAKE_O)
+       /\ ={b0, state_map}(Game2, Red_AEAD_real.WAKE_O)
        /\ Game2.dec_map{1} = GAEAD1.ctxts{2}
   ) Game2_inv_gen_pskey _ => //.
   proc.
@@ -1208,7 +1677,7 @@ call (:
 
 - conseq (: ={res}
        /\ ={psk_map}(Game2, GAEADb)
-       /\ ={state_map}(Game2, Red_AEAD.WAKE_O)
+       /\ ={b0, state_map}(Game2, Red_AEAD_real.WAKE_O)
        /\ Game2.dec_map{1} = GAEAD1.ctxts{2}
   ) Game2_inv_send_msg1 _ => //.
   proc; inline.
@@ -1219,7 +1688,7 @@ call (:
 
 - conseq (: ={res}
        /\ ={psk_map}(Game2, GAEADb)
-       /\ ={state_map}(Game2, Red_AEAD.WAKE_O)
+       /\ ={b0, state_map}(Game2, Red_AEAD_real.WAKE_O)
        /\ Game2.dec_map{1} = GAEAD1.ctxts{2}
   ) Game2_inv_send_msg2 _ => //.
   proc; inline.
@@ -1234,7 +1703,7 @@ call (:
 
 - conseq (: ={res}
        /\ ={psk_map}(Game2, GAEADb)
-       /\ ={state_map}(Game2, Red_AEAD.WAKE_O)
+       /\ ={b0, state_map}(Game2, Red_AEAD_real.WAKE_O)
        /\ Game2.dec_map{1} = GAEAD1.ctxts{2}
   ) Game2_inv_send_msg3 _ => //.
   proc; inline.
@@ -1259,7 +1728,7 @@ call (:
 
 - conseq (: ={res}
        /\ ={psk_map}(Game2, GAEADb)
-       /\ ={state_map}(Game2, Red_AEAD.WAKE_O)
+       /\ ={b0, state_map}(Game2, Red_AEAD_real.WAKE_O)
        /\ Game2.dec_map{1} = GAEAD1.ctxts{2}
   ) Game2_inv_send_fin _ => //.
   proc; inline.
@@ -1275,14 +1744,211 @@ call (:
 
 - conseq (: ={res}
        /\ ={psk_map}(Game2, GAEADb)
-       /\ ={state_map}(Game2, Red_AEAD.WAKE_O)
+       /\ ={b0, state_map}(Game2, Red_AEAD_real.WAKE_O)
        /\ Game2.dec_map{1} = GAEAD1.ctxts{2}
   ) Game2_inv_rev_skey _ => //.
   by sim.
 
 - conseq (: ={res}
        /\ ={psk_map}(Game2, GAEADb)
-       /\ ={state_map}(Game2, Red_AEAD.WAKE_O)
+       /\ ={b0, state_map}(Game2, Red_AEAD_real.WAKE_O)
+       /\ Game2.dec_map{1} = GAEAD1.ctxts{2}
+  ) Game2_inv_test _ => //.
+  by sim.
+
+auto=> /> a i.
+exact /Game1_undef/emptyE.
+qed.
+
+lemma Step1_ideal &m:
+    `|Pr[E_GWAKE(Game1, A).run(true) @ &m : res] - Pr[E_GWAKE(Game2, A).run(true) @ &m : res]|
+  = 
+    `|Pr[E_GAEAD(GAEAD0, Red_AEAD_ideal(A)).run() @ &m : res] - Pr[E_GAEAD(GAEAD1, Red_AEAD_ideal(A)).run() @ &m : res]|.
+proof.
+do! congr.
++ byequiv => //.
+  proc; inline*.
+  wp.
+  call (:
+        ={psk_map}(Game1, GAEADb)
+     /\ ={b0, state_map}(Game1, Red_AEAD_ideal.WAKE_O)
+     /\ (forall a i, Game1_inv Game1.state_map Game1.psk_map a i){1}
+  )=> //.
+
+  - conseq (: ={res}
+         /\ ={psk_map}(Game1, GAEADb)
+         /\ ={b0, state_map}(Game1, Red_AEAD_ideal.WAKE_O)
+    ) Game1_inv_gen_pskey _ => //.
+    by proc; if; auto.
+
+  - conseq (: ={res}
+         /\ ={psk_map}(Game1, GAEADb)
+         /\ ={b0, state_map}(Game1, Red_AEAD_ideal.WAKE_O)
+    ) Game1_inv_send_msg1 _ => //.
+    proc; inline.
+    sp; wp; if=> //.
+    by match Some {2} ^match; auto; smt().
+
+  - conseq (: ={res}
+         /\ ={psk_map}(Game1, GAEADb)
+         /\ ={b0, state_map}(Game1, Red_AEAD_ideal.WAKE_O)
+    ) Game1_inv_send_msg2 _ => //.
+    proc; inline.
+    sp; wp; if=> //.
+    match Some {2} ^match.
+    + auto; smt().
+    sp; match =.
+    + by move=> /> /#.
+    + by auto. 
+    move=> na.
+    by match Some {2} ^match; auto; smt().
+
+  - conseq (: ={res}
+         /\ ={psk_map}(Game1, GAEADb)
+         /\ ={b0, state_map}(Game1, Red_AEAD_ideal.WAKE_O)
+    ) Game1_inv_send_msg3 _ => //.
+    proc; inline.
+    sp; wp; if=> //.
+    sp; match = => //. 
+    + smt().
+    move=> st m1.
+    exlim Game1.state_map{1}, Game1.psk_map{1}, a{1}, i{1} => sm pm a i.
+    case @[ambient] _: (forall a i, Game1_inv sm pm a i) => [inv|?]; 2: by exfalso => /#. 
+    case @[ambient] _: (inv a i); 1,2,4,5,6: (move=> *; exfalso=> /#).
+    move=> b na c1 kab smai pmab.
+    match Some {2} ^match; 1: by auto=> /#.
+    sp; match =.
+    + by auto=> /> /#. 
+    + by auto=> /> /#.
+    move=> nb.
+    match Some {2} ^match; 1: by auto=> /#.
+    by auto=> /> /#.
+
+  - conseq (: ={res}
+         /\ ={psk_map}(Game1, GAEADb)
+         /\ ={b0, state_map}(Game1, Red_AEAD_ideal.WAKE_O)
+    ) Game1_inv_send_fin _ => //.
+    proc; inline.
+    sp; wp ^if ^if; if=> //.
+    sp; match = => //.
+    + move=> /#.
+    move=> st m1 m2.
+    match Some {2} ^match.
+    + auto=> />. 
+      move=> &hr smr sml invl bj_in.
+      by case: (invl b{m0} j{m0})=> /#.
+    by sp; match =; auto=> /> /#.
+
+  - conseq (: ={res}
+         /\ ={psk_map}(Game1, GAEADb)
+         /\ ={b0, state_map}(Game1, Red_AEAD_ideal.WAKE_O)
+    ) Game1_inv_rev_skey _ => //.
+    by sim.
+
+  - conseq (: ={res}
+         /\ ={psk_map}(Game1, GAEADb)
+         /\ ={b0, state_map}(Game1, Red_AEAD_ideal.WAKE_O)
+    ) Game1_inv_test _ => //.
+    by sim. 
+  
+  auto=> />.
+  move=> a i.
+  exact /Game1_undef/emptyE.
+
+byequiv => //.
+proc; inline*.
+wp.
+call (:
+      ={psk_map}(Game2, GAEADb)
+      /\ ={b0, state_map}(Game2, Red_AEAD_ideal.WAKE_O)
+      /\ Game2.dec_map{1} = GAEAD1.ctxts{2}
+      /\ (forall a i, Game1_inv Game2.state_map Game2.psk_map a i){1}
+).
+- conseq (: ={res}
+       /\ ={psk_map}(Game2, GAEADb)
+       /\ ={b0, state_map}(Game2, Red_AEAD_ideal.WAKE_O)
+       /\ Game2.dec_map{1} = GAEAD1.ctxts{2}
+  ) Game2_inv_gen_pskey _ => //.
+  proc.
+  by if; auto.
+
+- conseq (: ={res}
+       /\ ={psk_map}(Game2, GAEADb)
+       /\ ={b0, state_map}(Game2, Red_AEAD_ideal.WAKE_O)
+       /\ Game2.dec_map{1} = GAEAD1.ctxts{2}
+  ) Game2_inv_send_msg1 _ => //.
+  proc; inline.
+  sp; wp; if=> //.
+  rcondt{2} ^if; 1: by auto.
+  swap {2} ^c<$ @ ^na<$.
+  by auto.
+
+- conseq (: ={res}
+       /\ ={psk_map}(Game2, GAEADb)
+       /\ ={b0, state_map}(Game2, Red_AEAD_ideal.WAKE_O)
+       /\ Game2.dec_map{1} = GAEAD1.ctxts{2}
+  ) Game2_inv_send_msg2 _ => //.
+  proc; inline.
+  sp; wp; if=> //.
+  rcondt {2} 5; 1: by auto.
+  sp; match = => //.
+  + by auto.
+  move=> na.
+  rcondt {2} ^if; 1: by auto.
+  swap {2} ^c0<$ @ ^nb<$.
+  by auto.
+
+- conseq (: ={res}
+       /\ ={psk_map}(Game2, GAEADb)
+       /\ ={b0, state_map}(Game2, Red_AEAD_ideal.WAKE_O)
+       /\ Game2.dec_map{1} = GAEAD1.ctxts{2}
+  ) Game2_inv_send_msg3 _ => //.
+  proc; inline.
+  sp; wp; if=> //.
+  sp; match = => //.
+  + smt().
+  move=> st m1.
+  rcondt {2} ^if.
+  + auto=> />.
+    move=> &hr smr sml invl ai_in.
+    by case: (invl a{m0} i{m0})=> /#.
+  sp; match =.
+  + by auto.
+  + by auto.
+  move=> nb.
+  rcondt {2} ^if.
+  + auto=> />.
+    move=> &hr decl decr smr sml invl ai_in ok _.
+    by case: (invl a{m0} i{m0})=> /#.
+  swap {2} ^c0<$ @ ^ok<$.
+  by auto.
+
+- conseq (: ={res}
+       /\ ={psk_map}(Game2, GAEADb)
+       /\ ={b0, state_map}(Game2, Red_AEAD_ideal.WAKE_O)
+       /\ Game2.dec_map{1} = GAEAD1.ctxts{2}
+  ) Game2_inv_send_fin _ => //.
+  proc; inline.
+  sp; wp ^if ^if; if=> //.
+  sp; match = => //.
+  + smt().
+  move=> st m1 m2.
+  rcondt {2} 6.
+  + auto=> />.
+    move=> &hr smr sml invl ai_in.
+    by case: (invl b{m0} j{m0})=> /#.
+  by sp; match =; auto.
+
+- conseq (: ={res}
+       /\ ={psk_map}(Game2, GAEADb)
+       /\ ={b0, state_map}(Game2, Red_AEAD_ideal.WAKE_O)
+       /\ Game2.dec_map{1} = GAEAD1.ctxts{2}
+  ) Game2_inv_rev_skey _ => //.
+  by sim.
+
+- conseq (: ={res}
+       /\ ={psk_map}(Game2, GAEADb)
+       /\ ={b0, state_map}(Game2, Red_AEAD_ideal.WAKE_O)
        /\ Game2.dec_map{1} = GAEAD1.ctxts{2}
   ) Game2_inv_test _ => //.
   by sim.
@@ -1294,14 +1960,14 @@ qed.
 (* ------------------------------------------------------------------------------------------ *)
 (* Step 2a: Remove collisions of all produced ciphertexts. *)
 
-lemma Step2 &m: `| Pr[E_GWAKE(Game2, A).run() @ &m : res] - Pr[E_GWAKE(Game3, A).run() @ &m : res] | <= Pr[E_GWAKE(Game2, A).run() @ &m : Game2.bad].
+lemma Step2 bit &m: `| Pr[E_GWAKE(Game2, A).run(bit) @ &m : res] - Pr[E_GWAKE(Game3, A).run(bit) @ &m : res] | <= Pr[E_GWAKE(Game2, A).run(bit) @ &m : Game2.bad].
 proof.
 rewrite StdOrder.RealOrder.distrC.
 byequiv (: _ ==> _) : Game3.bad => //; first last.
 + move=> &1 &2.
   by case: (Game2.bad{2}).
 symmetry; proc; inline*.
-call (: Game3.bad, ={bad, psk_map, state_map, dec_map}(Game2, Game3), ={bad}(Game2, Game3)) => //.
+call (: Game3.bad, ={b0, bad, psk_map, state_map, dec_map}(Game2, Game3), ={bad}(Game2, Game3)) => //.
 + exact A_ll.
 
 + by proc; inline*; auto; if; auto.
@@ -1379,11 +2045,22 @@ call (: Game3.bad, ={bad, psk_map, state_map, dec_map}(Game2, Game3), ={bad}(Gam
 
 + proc.
   sp; wp ^if ^if; if=> //.
-  sp; match =; auto; smt(). 
+  sp; match =; auto. 
+  + smt().
+  sp; if => //; 1: by smt(). 
+  sp; if => //; if => //; auto => /#.
 + move=> &2 ->.
-  proc; sp; wp ^if; if=> //; sp; match =; auto; smt().
+  proc; sp; wp ^if; if=> //; sp; match =; auto.
+  sp; if => //; sp; if => //; if => //. 
+  + auto => /#. 
+  auto => />.
+  by rewrite dskey_ll.
 + move=> &1.
-  proc; sp; wp ^if; if=> //; sp; match =; auto; smt().
+  proc; sp; wp ^if; if=> //; sp; match =; auto.
+  sp; if => //; sp; if => //; if => //. 
+  + auto => /#. 
+  auto => />.
+  by rewrite dskey_ll.
 auto=> />.
 move=> rl rr al bl dl pl sl ar br dr pr sr. 
 by case : (!br) => />.
@@ -1392,10 +2069,13 @@ qed.
 (* ------------------------------------------------------------------------------------------ *)
 (* Step 2b: Bound the bad event. *)
 
-lemma Step2b &m: Pr[E_GWAKE(Game2, A).run() @ &m : Game2.bad] <= ((q_m1 + q_m2 + q_m3) ^ 2)%r * mu1 dctxt (mode dctxt).
+lemma Step2b bit &m: Pr[E_GWAKE(Game2, A).run(bit) @ &m : Game2.bad] <= ((q_m1 + q_m2 + q_m3) ^ 2)%r * mu1 dctxt (mode dctxt).
 proof.
-apply (StdOrder.RealOrder.ler_trans Pr[BD.Exp(BD.Sample, Red_Coll(A)).main() @ &m : !uniq BD.Sample.l]); first last.
-+ apply (BD.pr_collision_q2 (Red_Coll(A))).
+case (bit) => real_ideal.
+
+(* Proof for the ideal side *)
+apply (StdOrder.RealOrder.ler_trans Pr[BD.Exp(BD.Sample, Red_Coll_ideal(A)).main() @ &m : !uniq BD.Sample.l]); first last.
++ apply (BD.pr_collision_q2 (Red_Coll_ideal(A))).
   + move => S S_ll.
     islossless.
     apply (A_ll (Counter(Red_Coll_O_WAKE(S)))); islossless.
@@ -1432,13 +2112,99 @@ apply (StdOrder.RealOrder.ler_trans Pr[BD.Exp(BD.Sample, Red_Coll(A)).main() @ &
     auto => /#.
   + proc; inline*; auto => /#.
   + proc; inline*; auto => /#.
-  + proc; inline*; auto => /#.
+  + proc; inline*; sp; if => //; sp; match => //. 
+    sp; if => //; sp; if => //. if => //; auto => /#.
   auto=> /#.
 
 byequiv => //.
 proc; inline.
 call (:
- ={state_map, psk_map, bad, dec_map}(Game2, Red_Coll_O_WAKE(BD.Sample))
+ ={b0, state_map, psk_map, bad, dec_map}(Game2, Red_Coll_O_WAKE(BD.Sample))
+ /\ (Game2.bad{1} => !uniq BD.Sample.l{2})
+ /\ (forall c, (exists pk ad, (pk, ad, c) \in Red_Coll_O_WAKE.dec_map) => c \in BD.Sample.l){2}
+) => //.
+
++ by sim />.
+
++ proc; inline.
+  sp; if=> //; auto=> />.
+  smt(mem_set).
+
++ proc; inline.
+  sp; if=> //; 2: by auto=> />.
+  sp; match = => //.
+  + by auto => />.
+  move=> na.
+  auto=> />.
+  smt(mem_set).
+
++ proc; inline.
+  sp; if=> //; 2: by auto=> />.
+  sp; match =; auto=> />.
+  + smt().
+  + smt().
+  sp; match = => //.
+  + by auto=> /#.
+  move=> nb.
+  auto=> />.
+  smt(mem_set).
+
++ by sim />.
+
++ by sim />.
+
+by sim />.
+
+auto=> />.
+smt(emptyE).
+
+(* Proof for the real side *)
+apply (StdOrder.RealOrder.ler_trans Pr[BD.Exp(BD.Sample, Red_Coll_real(A)).main() @ &m : !uniq BD.Sample.l]); first last.
++ apply (BD.pr_collision_q2 (Red_Coll_real(A))).
+  + move => S S_ll.
+    islossless.
+    apply (A_ll (Counter(Red_Coll_O_WAKE(S)))); islossless.
+    + by match; auto; islossless.
+    + match; auto. 
+      by sp; match; auto; islossless.
+    + match => //.
+      by sp; match; auto; islossless.
+    match => //; islossless.
+    by match; islossless.
+  proc; inline.
+  sp.
+  conseq (: _ ==> size BD.Sample.l <= Counter.cm1 + Counter.cm2 + Counter.cm3) (: Counter.cm1 = 0 /\ Counter.cm2 = 0 /\ Counter.cm3 = 0 ==> Counter.cm1 <= q_m1 /\ Counter.cm2 <= q_m2 /\ Counter.cm3 <= q_m3)=> //.
+  + smt().
+  + by call (A_bounded_qs (Red_Coll_O_WAKE(BD.Sample))).
+  call (: size BD.Sample.l <= Counter.cm1 + Counter.cm2 + Counter.cm3) => //.
+  + proc; inline*; if; auto.
+  + proc; inline*; sp; if => //; auto => /#.
+  + proc; inline*.
+    sp; if => //.
+    + case ((Red_Coll_O_WAKE.dec_map.[(a, b), msg1_data a b, ca]) = None).
+      + match None ^match => //. 
+        auto => /#.
+      match Some ^match => //; auto => /#.
+    auto => /#.
+  + proc; inline*.
+    sp; if => //.
+    + sp; match; 2,3,4,5: auto => /#.
+      case ((Red_Coll_O_WAKE.dec_map.[(a, s.`1), msg2_data a s.`1 s.`4, m2]) = None).
+      + match None ^match => //.  
+        + by auto => />.
+        by auto => /#.
+      by match Some ^match => //; auto => /#.
+    auto => /#.
+  + proc; inline*; auto => /#.
+  + proc; inline*; auto => /#.
+  + proc; inline*; sp; if => //; sp; match => //. 
+    sp; if => //; sp; if => //. if => //; auto => /#.
+  auto=> /#.
+
+byequiv => //.
+proc; inline.
+call (:
+ ={b0, state_map, psk_map, bad, dec_map}(Game2, Red_Coll_O_WAKE(BD.Sample))
  /\ (Game2.bad{1} => !uniq BD.Sample.l{2})
  /\ (forall c, (exists pk ad, (pk, ad, c) \in Red_Coll_O_WAKE.dec_map) => c \in BD.Sample.l){2}
 ) => //.
@@ -1522,24 +2288,24 @@ case: (sml.[h])=> //.
 by move=> [r' []] // [].
 qed.
 
-lemma Step3 &m: Pr[E_GWAKE(Game3, A).run() @ &m : res] = Pr[E_GWAKE(Game4, A).run() @ &m :res].
+lemma Step3 bit &m: Pr[E_GWAKE(Game3, A).run(bit) @ &m : res] = Pr[E_GWAKE(Game4, A).run(bit) @ &m :res].
 proof.
-byequiv (: ={glob A} ==> _) => //.
+byequiv (: ={glob A, arg} ==> _) => //.
 proc; inline*.
-call(: ={psk_map, bad, dec_map}(Game3, Game4)
+call(: ={b0, psk_map, bad, dec_map}(Game3, Game4)
     /\ (forall h, omap (fun v => let (r, s) = v in (r, clear_nonces s)) Game3.state_map.[h]{1} = Game4.state_map.[h]{2})
     /\ (forall a i, Game3_inv Game3.state_map Game3.dec_map a i){1}
 ).
 
 - conseq (: ={res}
-    /\ ={psk_map, bad, dec_map}(Game3, Game4)
+    /\ ={b0, psk_map, bad, dec_map}(Game3, Game4)
     /\ (forall h, omap (fun v => let (r, s) = v in (r, clear_nonces s)) Game3.state_map.[h]{1} = Game4.state_map.[h]{2})
   ) Game3_inv_gen_pskey _ => //.
   proc.
   by if; auto.
 
 - conseq (: ={res}
-    /\ ={psk_map, bad, dec_map}(Game3, Game4)
+    /\ ={b0, psk_map, bad, dec_map}(Game3, Game4)
     /\ (forall h, omap (fun v => let (r, s) = v in (r, clear_nonces s)) Game3.state_map.[h]{1} = Game4.state_map.[h]{2})
   ) Game3_inv_send_msg1 _ => //.
   proc; inline*.
@@ -1552,7 +2318,7 @@ call(: ={psk_map, bad, dec_map}(Game3, Game4)
   smt(get_setE).
 
 - conseq (: ={res}
-    /\ ={psk_map, bad, dec_map}(Game3, Game4)
+    /\ ={b0, psk_map, bad, dec_map}(Game3, Game4)
     /\ (forall h, omap (fun v => let (r, s) = v in (r, clear_nonces s)) Game3.state_map.[h]{1} = Game4.state_map.[h]{2})
   ) Game3_inv_send_msg2 _ => //.
   proc; inline*.
@@ -1567,7 +2333,7 @@ call(: ={psk_map, bad, dec_map}(Game3, Game4)
   smt(get_setE).
 
 - conseq (: ={res}
-    /\ ={psk_map, bad, dec_map}(Game3, Game4)
+    /\ ={b0, psk_map, bad, dec_map}(Game3, Game4)
     /\ (forall h, omap (fun v => let (r, s) = v in (r, clear_nonces s)) Game3.state_map.[h]{1} = Game4.state_map.[h]{2})
   ) Game3_inv_send_msg3 _ => //.
   proc; inline*.
@@ -1592,7 +2358,7 @@ call(: ={psk_map, bad, dec_map}(Game3, Game4)
   by case: (invl a{2} i{2}); smt(get_setE).
 
 - conseq (: ={res}
-    /\ ={psk_map, bad, dec_map}(Game3, Game4)
+    /\ ={b0, psk_map, bad, dec_map}(Game3, Game4)
     /\ (forall h, omap (fun v => let (r, s) = v in (r, clear_nonces s)) Game3.state_map.[h]{1} = Game4.state_map.[h]{2})
   ) Game3_inv_send_fin _ => //.
   proc; inline*.
@@ -1614,7 +2380,7 @@ call(: ={psk_map, bad, dec_map}(Game3, Game4)
   move=> &1 &2 <- dm smr sml inv /(_ b{2} j{2}) []; smt(get_setE).
 
 - conseq (: ={res}
-    /\ ={psk_map, bad, dec_map}(Game3, Game4)
+    /\ ={b0, psk_map, bad, dec_map}(Game3, Game4)
     /\ (forall h, omap (fun v => let (r, s) = v in (r, clear_nonces s)) Game3.state_map.[h]{1} = Game4.state_map.[h]{2})
   ) Game3_inv_rev_skey _ => //.
   proc; inline. 
@@ -1643,7 +2409,7 @@ call(: ={psk_map, bad, dec_map}(Game3, Game4)
   do rewrite get_set_neqE => //. rewrite eqsm => //.
 
 - conseq (: ={res}
-    /\ ={psk_map, bad, dec_map}(Game3, Game4)
+    /\ ={b0, psk_map, bad, dec_map}(Game3, Game4)
     /\ (forall h, omap (fun v => let (r, s) = v in (r, clear_nonces s)) Game3.state_map.[h]{1} = Game4.state_map.[h]{2})
   ) Game3_inv_test _ => //.
   proc; inline. 
@@ -1662,13 +2428,20 @@ call(: ={psk_map, bad, dec_map}(Game3, Game4)
   sp ^if & -1 ^if & -1; if=> //.
   + move => &1 &2 [] /> *.
     by rewrite (eq_obs_partners_nonces (a, i){2} Game3.state_map{1} Game4.state_map{2}) => //.
-  auto=> /> &1 &2 + + eqsm invl a_in _.
+  if => //.
+  + auto=> /> &1 &2 + + eqsm invl a_in _.
+    rewrite -(eqsm (a, i){2}).
+    move => *.
+    split. smt().
+    move => h.
+    case (h = (a, i){2}) => [|hneq].
+    smt(get_set_sameE). 
+    do rewrite get_set_neqE => //. rewrite eqsm => //.
+  auto=> /> &1 &2 + + eqsm invl a_in _ _ ideal sk _.
   rewrite -(eqsm (a, i){2}).
-  move => *.
-  split. smt().
-  move => h.
+  move => stm1 stm2 h.
   case (h = (a, i){2}) => [|hneq].
-  smt(get_set_sameE). 
+  + smt(get_set_sameE). 
   do rewrite get_set_neqE => //. rewrite eqsm => //.
  
 auto=> />.
@@ -1685,15 +2458,18 @@ local clone import DProd.ProdSampling with
   type t2 <- nonce
 proof *.
 
-lemma Step4 &m: Pr[E_GWAKE(Game4, A).run() @ &m : res] = Pr[E_GWAKE(Game5, A).run() @ &m : res].
+lemma Step4 bit &m: Pr[E_GWAKE(Game4, A).run(bit) @ &m : res] = Pr[E_GWAKE(Game5, A).run(bit) @ &m : res].
 byequiv => //.
 proc*.
-transitivity* {1} { r <@ MainD(Red_ROM(A), RO).distinguish(); }.
+case (bit).
+
+(* Proof for the ideal side *)
+transitivity* {1} { r <@ MainD(Red_ROM_ideal(A), RO).distinguish(); }.
 
 + inline*.
   wp.
-  call (: ={state_map, psk_map, bad}(Game4, Red_ROM.WAKE_O)
-       /\ (forall h, h \in Game4.dec_map{1} <=> h \in Red_ROM.WAKE_O.dec_map{2})
+  call (: ={b0, state_map, psk_map, bad}(Game4, Red_ROM_ideal.WAKE_O)
+       /\ (forall h, h \in Game4.dec_map{1} <=> h \in Red_ROM_ideal.WAKE_O.dec_map{2})
        /\ (forall c ad n, (exists pk, Game4.dec_map{1}.[(pk, ad, c)] = Some n) <=> RO.m{2}.[(ad, c)] = Some n)
        /\ (forall a b ca cb, ((a, b), msg2_data a b ca, cb) \in Game4.dec_map => ((a, b), msg1_data a b, ca) \in Game4.dec_map){1}
        /\ (forall a b ca cb caf, ((a, b), msg3_data a b ca cb, caf) \in Game4.dec_map => ((a, b), msg2_data a b ca, cb) \in Game4.dec_map){1}
@@ -1769,10 +2545,10 @@ transitivity* {1} { r <@ MainD(Red_ROM(A), RO).distinguish(); }.
    auto=> />.
    smt(emptyE).
   
-rewrite equiv [{1} 1 (FullEager.RO_LRO (Red_ROM(A)) _)]; 1: by move=> _; exact dnonce_ll.
+rewrite equiv [{1} 1 (FullEager.RO_LRO (Red_ROM_ideal(A)) _)]; 1: by move=> _; exact dnonce_ll.
 inline*.
 wp; call (: 
-  ={state_map, psk_map, bad, dec_map}(Red_ROM.WAKE_O, Game5)
+  ={b0, state_map, psk_map, bad, dec_map}(Red_ROM_ideal.WAKE_O, Game5)
   /\ (forall a b ca, (forall cb caf, (msg3_data a b ca cb, caf) \notin Game5.prfkey_map{2})
         => (msg1_data a b, ca) \notin RO.m{1})
   /\ (forall a b ca cb, (forall caf, (msg3_data a b ca cb, caf) \notin Game5.prfkey_map{2})
@@ -1787,7 +2563,7 @@ wp; call (:
 - by sim />.
 
 - conseq (: ={res}
-  /\ ={state_map, psk_map, bad, dec_map}(Red_ROM.WAKE_O, Game5)
+  /\ ={b0, state_map, psk_map, bad, dec_map}(Red_ROM_ideal.WAKE_O, Game5)
   /\ (forall a b ca, (forall cb caf, (msg3_data a b ca cb, caf) \notin Game5.prfkey_map{2})
         => (msg1_data a b, ca) \notin RO.m{1})
   /\ (forall a b ca cb, (forall caf, (msg3_data a b ca cb, caf) \notin Game5.prfkey_map{2})
@@ -1802,7 +2578,7 @@ wp; call (:
   by auto=> />.
 
 - conseq (: ={res}
-  /\ ={state_map, psk_map, bad, dec_map}(Red_ROM.WAKE_O, Game5)
+  /\ ={b0, state_map, psk_map, bad, dec_map}(Red_ROM_ideal.WAKE_O, Game5)
   /\ (forall a b ca, (forall cb caf, (msg3_data a b ca cb, caf) \notin Game5.prfkey_map{2})
         => (msg1_data a b, ca) \notin RO.m{1})
   /\ (forall a b ca cb, (forall caf, (msg3_data a b ca cb, caf) \notin Game5.prfkey_map{2})
@@ -1817,7 +2593,7 @@ wp; call (:
   by sp; match =; auto=> />.
 
 - conseq (: ={res}
-  /\ ={state_map, psk_map, bad, dec_map}(Red_ROM.WAKE_O, Game5)
+  /\ ={b0, state_map, psk_map, bad, dec_map}(Red_ROM_ideal.WAKE_O, Game5)
   /\ (forall a b ca, (forall cb caf, (msg3_data a b ca cb, caf) \notin Game5.prfkey_map{2})
         => (msg1_data a b, ca) \notin RO.m{1})
   /\ (forall a b ca cb, (forall caf, (msg3_data a b ca cb, caf) \notin Game5.prfkey_map{2})
@@ -1851,7 +2627,7 @@ wp; call (:
     case: (invr5 a{m0} i{m0}) ; rewrite sms //=.
     move=> /> 4!->> _.
     rewrite mem_set /#.
-  outline {2} [3] (na, nb') <@ S.sample. 
+  outline {2} 3 by {(na, nb') <@ S.sample(dnonce, dnonce);}. 
   wp; rewrite equiv [{2} 3 sample_sample2].
   inline*.
   auto=> />.
@@ -1862,7 +2638,7 @@ wp; call (:
   smt(get_setE).
 
 - conseq (: ={res}
-  /\ ={state_map, psk_map, bad, dec_map}(Red_ROM.WAKE_O, Game5)
+  /\ ={b0, state_map, psk_map, bad, dec_map}(Red_ROM_ideal.WAKE_O, Game5)
   /\ (forall a b ca, (forall cb caf, (msg3_data a b ca cb, caf) \notin Game5.prfkey_map{2})
         => (msg1_data a b, ca) \notin RO.m{1})
   /\ (forall a b ca cb, (forall caf, (msg3_data a b ca cb, caf) \notin Game5.prfkey_map{2})
@@ -1896,7 +2672,7 @@ wp; call (:
   smt().
 
 - conseq (: ={res}
-  /\ ={state_map, psk_map, bad, dec_map}(Red_ROM.WAKE_O, Game5)
+  /\ ={b0, state_map, psk_map, bad, dec_map}(Red_ROM_ideal.WAKE_O, Game5)
   /\ (forall a b ca, (forall cb caf, (msg3_data a b ca cb, caf) \notin Game5.prfkey_map{2})
         => (msg1_data a b, ca) \notin RO.m{1})
   /\ (forall a b ca cb, (forall caf, (msg3_data a b ca cb, caf) \notin Game5.prfkey_map{2})
@@ -1909,7 +2685,245 @@ wp; call (:
   by sim />.
 
 - conseq (: ={res}
-  /\ ={state_map, psk_map, bad, dec_map}(Red_ROM.WAKE_O, Game5)
+  /\ ={b0, state_map, psk_map, bad, dec_map}(Red_ROM_ideal.WAKE_O, Game5)
+  /\ (forall a b ca, (forall cb caf, (msg3_data a b ca cb, caf) \notin Game5.prfkey_map{2})
+        => (msg1_data a b, ca) \notin RO.m{1})
+  /\ (forall a b ca cb, (forall caf, (msg3_data a b ca cb, caf) \notin Game5.prfkey_map{2})
+        => (msg2_data a b ca, cb) \notin RO.m{1})
+  /\ (forall a b ca cb caf, (msg3_data a b ca cb, caf) \in Game5.prfkey_map{2} =>
+         exists na nb, Game5.prfkey_map{2}.[(msg3_data a b ca cb, caf)] = Some (na, nb) /\
+                       RO.m{1}.[(msg1_data a b, ca)] = Some na /\
+                       RO.m{1}.[(msg2_data a b ca, cb)] = Some nb)
+  ) _ Game5_inv_test => //.
+  by sim />.
+
+auto => />.
+smt(Game5_undef emptyE).
+
+
+(* Proof for the real side *)
+transitivity* {1} { r <@ MainD(Red_ROM_real(A), RO).distinguish(); }.
+
++ inline*.
+  wp.
+  call (: ={b0, state_map, psk_map, bad}(Game4, Red_ROM_real.WAKE_O)
+       /\ (forall h, h \in Game4.dec_map{1} <=> h \in Red_ROM_real.WAKE_O.dec_map{2})
+       /\ (forall c ad n, (exists pk, Game4.dec_map{1}.[(pk, ad, c)] = Some n) <=> RO.m{2}.[(ad, c)] = Some n)
+       /\ (forall a b ca cb, ((a, b), msg2_data a b ca, cb) \in Game4.dec_map => ((a, b), msg1_data a b, ca) \in Game4.dec_map){1}
+       /\ (forall a b ca cb caf, ((a, b), msg3_data a b ca cb, caf) \in Game4.dec_map => ((a, b), msg2_data a b ca, cb) \in Game4.dec_map){1}
+  ) => //.
+
+  - by proc; sp; if; auto.
+
+  - proc; inline*.
+    sp; wp; if=> //.
+    seq 1 1 : (#pre /\ ={ca}); 1: by auto.
+    sp; if=> //.
+    + smt().
+    + rcondt {2} ^if; 1: by auto=> /#. 
+      auto=> />.
+      smt(get_setE).
+    by auto=> /#.
+  
+   - proc; inline*.
+     sp; wp; if=> //. 
+     match; 1,2: smt().
+     + by auto=> />.
+     move=> nal nar.
+     seq 1 1 : (#pre /\ ={cb}); 1: by auto.
+     sp; if=> //.
+     + smt().
+     + rcondt {2} ^if; 1: by auto=> /#. 
+       auto=> />.
+       smt(get_setE).
+     by auto=> /#.
+
+   - proc; inline*.
+     sp; wp; if=> //. 
+     sp; match = => //.
+     + smt().
+     move=> s m1.
+     sp; match; 1: smt().
+     + move => /> *; smt().
+     + by auto=> />.
+     move=> nbl nbr.
+     seq 1 1 : (#pre /\ ={caf}); 1: by auto.
+     sp; if=> //.
+     + smt().
+     + rcondt {2} ^if; 1: by auto=> /#.
+       rcondf {2} ^if.
+       + auto=> />.
+         smt(mem_set).
+       rcondf {2} ^if.
+       + auto=> />.
+         smt(mem_set).
+       swap {2} ^r1<$ @ ^ok<-.
+       seq 1 1 : (#pre /\ ok{1} = r1{2}); 1: by auto => />.
+       auto=> />.
+       smt(get_setE).
+    by auto=> /#.
+  
+   - proc; inline*.
+     sp; wp ^if ^if; if=> //. 
+     sp; match = => //.
+     + smt().
+     move=> s m1 m2.
+     sp; match; 1,2: smt().
+     + by auto=> />.
+     move=> nokl nokr.
+     rcondf {2} ^if; 1: by auto=> /#.
+     rcondf {2} ^if; 1: by auto=> /#.
+     auto=> />.
+     smt(get_setE).
+  
+   - by sim />.
+   
+   - by sim />.
+
+   auto=> />.
+   smt(emptyE).
+  
+rewrite equiv [{1} 1 (FullEager.RO_LRO (Red_ROM_real(A)) _)]; 1: by move=> _; exact dnonce_ll.
+inline*.
+wp; call (: 
+  ={b0, state_map, psk_map, bad, dec_map}(Red_ROM_real.WAKE_O, Game5)
+  /\ (forall a b ca, (forall cb caf, (msg3_data a b ca cb, caf) \notin Game5.prfkey_map{2})
+        => (msg1_data a b, ca) \notin RO.m{1})
+  /\ (forall a b ca cb, (forall caf, (msg3_data a b ca cb, caf) \notin Game5.prfkey_map{2})
+        => (msg2_data a b ca, cb) \notin RO.m{1})
+  /\ (forall a b ca cb caf, (msg3_data a b ca cb, caf) \in Game5.prfkey_map{2} =>
+         exists na nb, Game5.prfkey_map{2}.[(msg3_data a b ca cb, caf)] = Some (na, nb) /\
+                       RO.m{1}.[(msg1_data a b, ca)] = Some na /\
+                       RO.m{1}.[(msg2_data a b ca, cb)] = Some nb)
+  /\ (Game5_inv_full Game5.state_map Game5.dec_map Game5.prfkey_map){2}
+) => //.
+
+- by sim />.
+
+- conseq (: ={res}
+  /\ ={b0, state_map, psk_map, bad, dec_map}(Red_ROM_real.WAKE_O, Game5)
+  /\ (forall a b ca, (forall cb caf, (msg3_data a b ca cb, caf) \notin Game5.prfkey_map{2})
+        => (msg1_data a b, ca) \notin RO.m{1})
+  /\ (forall a b ca cb, (forall caf, (msg3_data a b ca cb, caf) \notin Game5.prfkey_map{2})
+        => (msg2_data a b ca, cb) \notin RO.m{1})
+  /\ (forall a b ca cb caf, (msg3_data a b ca cb, caf) \in Game5.prfkey_map{2} =>
+         exists na nb, Game5.prfkey_map{2}.[(msg3_data a b ca cb, caf)] = Some (na, nb) /\
+                       RO.m{1}.[(msg1_data a b, ca)] = Some na /\
+                       RO.m{1}.[(msg2_data a b ca, cb)] = Some nb)
+  ) _ Game5_inv_send_msg1 => //.
+  proc; inline*.
+  sp; wp; if=> //.
+  by auto=> />.
+
+- conseq (: ={res}
+  /\ ={b0, state_map, psk_map, bad, dec_map}(Red_ROM_real.WAKE_O, Game5)
+  /\ (forall a b ca, (forall cb caf, (msg3_data a b ca cb, caf) \notin Game5.prfkey_map{2})
+        => (msg1_data a b, ca) \notin RO.m{1})
+  /\ (forall a b ca cb, (forall caf, (msg3_data a b ca cb, caf) \notin Game5.prfkey_map{2})
+        => (msg2_data a b ca, cb) \notin RO.m{1})
+  /\ (forall a b ca cb caf, (msg3_data a b ca cb, caf) \in Game5.prfkey_map{2} =>
+         exists na nb, Game5.prfkey_map{2}.[(msg3_data a b ca cb, caf)] = Some (na, nb) /\
+                       RO.m{1}.[(msg1_data a b, ca)] = Some na /\
+                       RO.m{1}.[(msg2_data a b ca, cb)] = Some nb)
+  ) _ Game5_inv_send_msg2 => //.
+  proc; inline*.
+  sp; wp; if=> //.
+  by sp; match =; auto=> />.
+
+- conseq (: ={res}
+  /\ ={b0, state_map, psk_map, bad, dec_map}(Red_ROM_real.WAKE_O, Game5)
+  /\ (forall a b ca, (forall cb caf, (msg3_data a b ca cb, caf) \notin Game5.prfkey_map{2})
+        => (msg1_data a b, ca) \notin RO.m{1})
+  /\ (forall a b ca cb, (forall caf, (msg3_data a b ca cb, caf) \notin Game5.prfkey_map{2})
+        => (msg2_data a b ca, cb) \notin RO.m{1})
+  /\ (forall a b ca cb caf, (msg3_data a b ca cb, caf) \in Game5.prfkey_map{2} =>
+         exists na nb, Game5.prfkey_map{2}.[(msg3_data a b ca cb, caf)] = Some (na, nb) /\
+                       RO.m{1}.[(msg1_data a b, ca)] = Some na /\
+                       RO.m{1}.[(msg2_data a b ca, cb)] = Some nb)
+  ) _ Game5_inv_send_msg3 => //.
+  proc; inline*.
+  sp; wp; if=> //.
+  sp; match = => //.
+  + smt().
+  move=> s m1.
+  sp; match = => //.
+  + by auto.
+  move=> nb.
+  seq 1 1 : (#pre /\ ={caf}); 1: by auto.
+  sp; if=> //.
+  rcondt {1} ^if.
+  + auto=> />.
+    move=> &hr _ dm _ sm _ inv1 inv2 inv3 invr1 invr2 invr3 invr4 invr5 /domE/some_oget sms /negb_or [_ cafnin] r _. 
+    rewrite -sm in sms.
+    case: (invr5 a{m0} i{m0}); rewrite sms //=.
+    move=> /> 4!->> _.
+    exact inv1.
+  rcondt {1} ^if.
+  + auto=> />.
+    move=> &hr _ dm _ sm _ inv1 inv2 inv3 invr1 invr2 invr3 invr4 invr5 /domE/some_oget sms /negb_or [_ cafnin] r _ r1 _. 
+    rewrite -sm in sms.
+    case: (invr5 a{m0} i{m0}) ; rewrite sms //=.
+    move=> /> 4!->> _.
+    rewrite mem_set /#.
+  outline {2} 3 by {(na, nb') <@ S.sample(dnonce, dnonce);}. 
+  wp; rewrite equiv [{2} 3 sample_sample2].
+  inline*.
+  auto=> />.
+  move=> &1 &2 _ dm _ sm _ inv1 inv2 inv3 invr1 invr2 invr3 invr4 invr5 /domE/some_oget sms /negb_or [_ cafnin] r _ r1 _. 
+  rewrite get_set_sameE //=.
+  rewrite -sm in sms.
+  case: (invr5 a{2} i{2}); rewrite sms //=.
+  smt(get_setE).
+
+- conseq (: ={res}
+  /\ ={b0, state_map, psk_map, bad, dec_map}(Red_ROM_real.WAKE_O, Game5)
+  /\ (forall a b ca, (forall cb caf, (msg3_data a b ca cb, caf) \notin Game5.prfkey_map{2})
+        => (msg1_data a b, ca) \notin RO.m{1})
+  /\ (forall a b ca cb, (forall caf, (msg3_data a b ca cb, caf) \notin Game5.prfkey_map{2})
+        => (msg2_data a b ca, cb) \notin RO.m{1})
+  /\ (forall a b ca cb caf, (msg3_data a b ca cb, caf) \in Game5.prfkey_map{2} =>
+         exists na nb, Game5.prfkey_map{2}.[(msg3_data a b ca cb, caf)] = Some (na, nb) /\
+                       RO.m{1}.[(msg1_data a b, ca)] = Some na /\
+                       RO.m{1}.[(msg2_data a b ca, cb)] = Some nb)
+  ) _ Game5_inv_send_fin => //.
+- proc; inline*.
+  sp; wp ^if ^if; if=> //.
+  sp; match = => //.
+  + smt().
+  move=> s m1 m2.
+  sp; match = => //.
+  + by auto.
+  move=> nok.
+  rcondf {1} ^if.
+  + auto=> />.
+    move=> &hr dm _ sm _ inv1 inv2 inv3 invr1 invr2 invr3 invr4 invr5 /domE/some_oget sms r _.
+    rewrite -sm in sms.
+    case: (invr5 b{m0} j{m0}) ; rewrite sms //=.
+    smt().
+  rcondf {1} ^if.
+  + auto=> />.
+    move=> &hr dm _ sm _ inv1 inv2 inv3 invr1 invr2 invr3 invr4 invr5 /domE/some_oget sms r _ r2 _.
+    rewrite -sm in sms.
+    case: (invr5 b{m0} j{m0}) ; rewrite sms //=.
+    smt().
+  auto=> />.
+  smt().
+
+- conseq (: ={res}
+  /\ ={b0, state_map, psk_map, bad, dec_map}(Red_ROM_real.WAKE_O, Game5)
+  /\ (forall a b ca, (forall cb caf, (msg3_data a b ca cb, caf) \notin Game5.prfkey_map{2})
+        => (msg1_data a b, ca) \notin RO.m{1})
+  /\ (forall a b ca cb, (forall caf, (msg3_data a b ca cb, caf) \notin Game5.prfkey_map{2})
+        => (msg2_data a b ca, cb) \notin RO.m{1})
+  /\ (forall a b ca cb caf, (msg3_data a b ca cb, caf) \in Game5.prfkey_map{2} =>
+         exists na nb, Game5.prfkey_map{2}.[(msg3_data a b ca cb, caf)] = Some (na, nb) /\
+                       RO.m{1}.[(msg1_data a b, ca)] = Some na /\
+                       RO.m{1}.[(msg2_data a b ca, cb)] = Some nb)
+  ) _ Game5_inv_rev_skey => //.
+  by sim />.
+
+- conseq (: ={res}
+  /\ ={b0, state_map, psk_map, bad, dec_map}(Red_ROM_real.WAKE_O, Game5)
   /\ (forall a b ca, (forall cb caf, (msg3_data a b ca cb, caf) \notin Game5.prfkey_map{2})
         => (msg1_data a b, ca) \notin RO.m{1})
   /\ (forall a b ca cb, (forall caf, (msg3_data a b ca cb, caf) \notin Game5.prfkey_map{2})
@@ -1925,21 +2939,21 @@ auto => />.
 smt(Game5_undef emptyE).
 qed.
 
+
 (* ------------------------------------------------------------------------------------------ *)
 (* Step 5: Apply the PRF assumption. *)
 
-
-lemma Step5 &m:
-    `|Pr[E_GWAKE(Game5, A).run() @ &m : res] - Pr[E_GWAKE(Game6, A).run() @ &m : res]|
+lemma Step5_real &m:
+    `|Pr[E_GWAKE(Game5, A).run(false) @ &m : res] - Pr[E_GWAKE(Game6, A).run(false) @ &m : res]|
   = 
-    `|Pr[E_GPRF(PRF0, Red_PRF(A)).run() @ &m : res] - Pr[E_GPRF(PRF1, Red_PRF(A)).run() @ &m : res]|.
+    `|Pr[E_GPRF(PRF0, Red_PRF_real(A)).run() @ &m : res] - Pr[E_GPRF(PRF1, Red_PRF_real(A)).run() @ &m : res]|.
 proof.
 do! congr.
 + byequiv => //.
   proc; inline*.
   wp.
   call (:
-        ={psk_map, state_map, dec_map, bad}(Game5, Red_PRF.WAKE_O)
+        ={b0, psk_map, state_map, dec_map, bad}(Game5, Red_PRF_real.WAKE_O)
      /\ ={prfkey_map}(Game5, PRFb)
      /\ (Game5_inv_full Game5.state_map Game5.dec_map Game5.prfkey_map){1}
   )=> //.
@@ -1947,19 +2961,19 @@ do! congr.
   - by sim />.
 
   - conseq (: ={res}
-     /\ ={psk_map, state_map, dec_map, bad}(Game5, Red_PRF.WAKE_O)
+     /\ ={psk_map, state_map, dec_map, bad}(Game5, Red_PRF_real.WAKE_O)
      /\ ={prfkey_map}(Game5, PRFb)
     ) Game5_inv_send_msg1 _ => //.
     by sim />.
 
   - conseq (: ={res}
-     /\ ={psk_map, state_map, dec_map, bad}(Game5, Red_PRF.WAKE_O)
+     /\ ={psk_map, state_map, dec_map, bad}(Game5, Red_PRF_real.WAKE_O)
      /\ ={prfkey_map}(Game5, PRFb)
     ) Game5_inv_send_msg2 _ => //.
     by sim />.
 
   - conseq (: ={res}
-     /\ ={psk_map, state_map, dec_map, bad}(Game5, Red_PRF.WAKE_O)
+     /\ ={psk_map, state_map, dec_map, bad}(Game5, Red_PRF_real.WAKE_O)
      /\ ={prfkey_map}(Game5, PRFb)
     ) Game5_inv_send_msg3 _ => //.
     proc; inline*.
@@ -1982,7 +2996,7 @@ do! congr.
     smt(get_setE).
 
   - conseq (: ={res}
-     /\ ={psk_map, state_map, dec_map, bad}(Game5, Red_PRF.WAKE_O)
+     /\ ={psk_map, state_map, dec_map, bad}(Game5, Red_PRF_real.WAKE_O)
      /\ ={prfkey_map}(Game5, PRFb)
     ) Game5_inv_send_fin _ => //.
      proc; inline*.
@@ -2001,13 +3015,13 @@ do! congr.
      smt(get_setE).
 
   - conseq (: ={res}
-     /\ ={psk_map, state_map, dec_map, bad}(Game5, Red_PRF.WAKE_O)
+     /\ ={psk_map, state_map, dec_map, bad}(Game5, Red_PRF_real.WAKE_O)
      /\ ={prfkey_map}(Game5, PRFb)
     ) Game5_inv_rev_skey _ => //.
     by sim />.
 
   - conseq (: ={res}
-     /\ ={psk_map, state_map, dec_map, bad}(Game5, Red_PRF.WAKE_O)
+     /\ ={psk_map, state_map, dec_map, bad}(Game5, Red_PRF_real.WAKE_O)
      /\ ={prfkey_map}(Game5, PRFb)
     ) Game5_inv_test _ => //.
     by sim />.
@@ -2019,7 +3033,168 @@ byequiv => //.
 proc; inline *.
 wp.
 call (:
-      ={psk_map, state_map, dec_map, bad}(Game6, Red_PRF.WAKE_O)
+      ={b0, psk_map, state_map, dec_map, bad}(Game6, Red_PRF_real.WAKE_O)
+   /\ ={prfkey_map}(Game6, PRFb)
+   /\ (forall a b m1 m2 m3, ((a, b), msg3_data a b m1 m2, m3) \in Game6.dec_map{1} <=> ((msg3_data a b m1 m2, m3), (a, b)) \in PRF1.cache{2})
+   /\ (forall a b m1 m2 m3 k, PRF1.cache.[((msg3_data a b m1 m2, m3), (a, b))]{2} = Some k => Game6.sk_map.[((a, m1), m2, m3)]{1} = Some k)
+   /\ (forall a b m1 m2 m3, ((a, b), msg3_data a b m1 m2, m3) \in Game6.dec_map <=> (msg3_data a b m1 m2, m3) \in Game6.prfkey_map){1}
+)=> //. 
+
+- by sim />.
+
+- proc; inline*. 
+  sp; wp; if => //.
+  auto => />.
+  smt(get_setE).
+
+- proc; inline*.
+  sp; wp; if => //.
+  match = => //.
+  + by auto => />. 
+  auto => />.
+  smt(get_setE).
+
+- proc; inline*.
+  sp; wp; if=> //. 
+  sp; match = => //.
+  + smt().
+  move=> s m1.
+  sp; match =.
+  + smt().
+  + by auto=> />.
+  move=> nb.
+  seq 1 1 : (#pre /\ ={caf}); 1: by auto.
+  sp; if=> //.
+  rcondt{2} ^if.
+  + auto=> />.
+    smt().
+  match Some {2} ^match.
+  + auto=> />.
+    smt(get_setE). 
+  rcondt{2} ^if.
+  + auto => />.
+    smt().
+  auto=> />.
+  smt(get_setE).
+
+- proc; inline*.
+  sp; wp ^if ^if; if=> //. 
+  sp; match = => //.
+  + smt().
+  move=> s m1 m2.
+  sp; match =.
+  + smt().
+  + by auto=> />.
+  move=> nok.
+  match Some {2} ^match.
+  + auto=> />.
+    smt().
+  rcondf{2} ^if.
+  + auto => />.
+    smt().
+  auto=> />.
+  smt().
+
+- by sim />.
+
+- by sim />.
+
+auto => />.
+smt(emptyE).
+qed.
+
+
+lemma Step5_ideal &m:
+    `|Pr[E_GWAKE(Game5, A).run(true) @ &m : res] - Pr[E_GWAKE(Game6, A).run(true) @ &m : res]|
+  = 
+    `|Pr[E_GPRF(PRF0, Red_PRF_ideal(A)).run() @ &m : res] - Pr[E_GPRF(PRF1, Red_PRF_ideal(A)).run() @ &m : res]|.
+proof.
+do! congr.
++ byequiv => //.
+  proc; inline*.
+  wp.
+  call (:
+        ={b0, psk_map, state_map, dec_map, bad}(Game5, Red_PRF_ideal.WAKE_O)
+     /\ ={prfkey_map}(Game5, PRFb)
+     /\ (Game5_inv_full Game5.state_map Game5.dec_map Game5.prfkey_map){1}
+  )=> //.
+
+  - by sim />.
+
+  - conseq (: ={res}
+     /\ ={psk_map, state_map, dec_map, bad}(Game5, Red_PRF_ideal.WAKE_O)
+     /\ ={prfkey_map}(Game5, PRFb)
+    ) Game5_inv_send_msg1 _ => //.
+    by sim />.
+
+  - conseq (: ={res}
+     /\ ={psk_map, state_map, dec_map, bad}(Game5, Red_PRF_ideal.WAKE_O)
+     /\ ={prfkey_map}(Game5, PRFb)
+    ) Game5_inv_send_msg2 _ => //.
+    by sim />.
+
+  - conseq (: ={res}
+     /\ ={psk_map, state_map, dec_map, bad}(Game5, Red_PRF_ideal.WAKE_O)
+     /\ ={prfkey_map}(Game5, PRFb)
+    ) Game5_inv_send_msg3 _ => //.
+    proc; inline*.
+    sp; wp; if=> //. 
+    sp; match = => //.
+    + smt().
+    move=> s m1.
+    sp; match =.
+    + smt().
+    + by auto=> />.
+    move=> nb.
+    seq 1 1 : (#pre /\ ={caf}); 1: by auto.
+    sp; if=> //.
+    rcondt{2} ^if.
+    + auto=> />. 
+      smt().
+    match Some {2} ^match.
+    + by auto => />; smt(mem_set get_setE).
+    auto => />. 
+    smt(get_setE).
+
+  - conseq (: ={res}
+     /\ ={psk_map, state_map, dec_map, bad}(Game5, Red_PRF_ideal.WAKE_O)
+     /\ ={prfkey_map}(Game5, PRFb)
+    ) Game5_inv_send_fin _ => //.
+     proc; inline*.
+     sp; wp ^if ^if; if=> //. 
+     sp; match = => //.
+     + smt().
+     move=> s m1 m2.
+     sp; match =.
+     + smt().
+     + by auto=> />.
+     move=> nok.
+     match Some {2} ^match.
+     + auto=> />.
+       smt().
+     auto => />.
+     smt(get_setE).
+
+  - conseq (: ={res}
+     /\ ={psk_map, state_map, dec_map, bad}(Game5, Red_PRF_ideal.WAKE_O)
+     /\ ={prfkey_map}(Game5, PRFb)
+    ) Game5_inv_rev_skey _ => //.
+    by sim />.
+
+  - conseq (: ={res}
+     /\ ={psk_map, state_map, dec_map, bad}(Game5, Red_PRF_ideal.WAKE_O)
+     /\ ={prfkey_map}(Game5, PRFb)
+    ) Game5_inv_test _ => //.
+    by sim />.
+
+  auto => />.
+  smt(emptyE Game5_undef).
+
+byequiv => //.
+proc; inline *.
+wp.
+call (:
+      ={b0, psk_map, state_map, dec_map, bad}(Game6, Red_PRF_ideal.WAKE_O)
    /\ ={prfkey_map}(Game6, PRFb)
    /\ (forall a b m1 m2 m3, ((a, b), msg3_data a b m1 m2, m3) \in Game6.dec_map{1} <=> ((msg3_data a b m1 m2, m3), (a, b)) \in PRF1.cache{2})
    /\ (forall a b m1 m2 m3 k, PRF1.cache.[((msg3_data a b m1 m2, m3), (a, b))]{2} = Some k => Game6.sk_map.[((a, m1), m2, m3)]{1} = Some k)
@@ -2127,13 +3302,13 @@ case: (sml.[h])=> //.
 by move=> [r' []] // [].
 qed.
 
-lemma Step6 &m:
-    Pr[E_GWAKE(Game6, A).run() @ &m : res] = Pr[E_GWAKE(Game7, A).run() @ &m : res].
+lemma Step6 bit &m:
+    Pr[E_GWAKE(Game6, A).run(bit) @ &m : res] = Pr[E_GWAKE(Game7, A).run(bit) @ &m : res].
 proof.
 byequiv => //.
 proc; inline*.
 call (:
-    ={psk_map, dec_map, bad, prfkey_map, sk_map}(Game6, Game7)
+    ={b0, psk_map, dec_map, bad, prfkey_map, sk_map}(Game6, Game7)
 /\ (forall h, omap (fun v => let (r, s) = v in (r, clear_sk s)) Game6.state_map.[h]{1} = Game7.state_map.[h]{2})
 /\ (forall h r tr k, Game6.state_map.[h] = Some (r, Accepted tr k) => Game6.sk_map.[tr] = Some k){1}
 /\ (forall a b m1 m2 m3, ((a, b), msg3_data a b m1 m2, m3) \in Game6.dec_map => ((a, m1), m2, m3) \in Game6.sk_map){1}
@@ -2216,14 +3391,23 @@ call (:
   sp ^if & -1 ^if & -1; if=> //.
   + move => &1 &2 [] /> *.
     by rewrite (eq_obs_partners_sk (a, i){2} Game6.state_map{1} Game7.state_map{2}) => //.
-  auto=> /> &1 &2 + + eqsm invl a_in _.
+  if => //.  
+  + auto=> /> &1 &2 + + eqsm invl a_in _.
+    rewrite -(eqsm (a, i){2}).
+    move => *.
+    split. smt().
+    split.
+    move => h.
+    case (h = (a, i){2}) => [|hneq].
+    + smt(get_set_sameE). 
+    do rewrite get_set_neqE => //. rewrite eqsm => //.
+    smt(get_setE).
+  auto=> /> &1 &2 + + eqsm invl a_in _ _ _ _ ideal sk _.
   rewrite -(eqsm (a, i){2}).
-  move => *.
-  split. smt().
-  split.
-  move => h.
+  move => stm1 stm2.
+  split. move => h.
   case (h = (a, i){2}) => [|hneq].
-  smt(get_set_sameE). 
+  + smt(get_set_sameE). 
   do rewrite get_set_neqE => //. rewrite eqsm => //.
   smt(get_setE).
 
